theories/iris_extra/saved_interp_n.v
@@ -1,22 +1,34 @@
-From iris.proofmode Require Import tactics.
 From iris.base_logic Require Import lib.saved_prop.
+From D Require Import prelude iris_prelude asubst_intf.
 
 (** saved interpretations *)
+Module Type SavedInterpN (Import V : VlSortsSig).
 
-Notation savedPred3G Σ A B C := (savedPredG Σ (A * B * C)).
-Notation savedPred3Σ A B C := (savedPredΣ (A * B * C)).
+Notation envPred s Σ := (env -d> s -d> iPropO Σ).
+Notation envD Σ := (envPred vl Σ).
+
+Definition hoEnvPred s Σ := list vl -d> envPred s Σ.
+Notation hoEnvD := (hoEnvPred vl).
+
+Definition hoD Σ := (* HO args *) list vl -d> vl -d> iPropO Σ.
+(* Definition packedHoEnvD Σ := packedHoEnvPred vl Σ. *)
+(* TODO name*)
+Local Notation argType s := (list vl * env * s)%type.
+
+Notation savedHoEnvPredG s Σ := (savedPredG Σ (argType s)).
+Notation savedHoEnvPredΣ s := (savedPredΣ (argType s)).
 
 Section saved_pred3.
-  Context {A B C : Type}.
-  Context `{!savedPred3G Σ A B C}.
-  Implicit Type (Φ : A -d> B -d> C -d> iPropO Σ).
+  Context {s : Type}.
+  Context `{!savedHoEnvPredG s Σ}.
+  Implicit Type (Φ : list vl -d> env -d> s -d> iPropO Σ).
 
-  Definition curryC Φ : A * B * C -d> iPropO Σ := (λ '(a, b, c), Φ a b c).
+  Definition curryC Φ : argType s -d> iPropO Σ := (λ '(a, b, c), Φ a b c).
 
   Definition saved_pred3_own (γ : gname) Φ :=
     saved_pred_own γ (curryC Φ).
 
-  Instance saved_pred3_own_contractive γ : Contractive (saved_pred3_own γ).
+  #[global] Instance saved_pred3_own_contractive γ : Contractive (saved_pred3_own γ).
   Proof.
     rewrite /saved_pred3_own => n f g Hfg.
     apply saved_pred_own_contractive. case: n Hfg => [//|n Hfg [[]] //].
@@ -33,7 +45,18 @@ Section saved_pred3.
   Proof. apply (saved_pred_agree γ (curryC Φ) (curryC Ψ) (a, b, c)). Qed.
 End saved_pred3.
 
+Typeclasses Opaque saved_pred3_own.
 #[global] Opaque saved_pred3_own.
 
-(* XXX solve notation overlap. *)
 Notation "γ ⤇ φ" := (saved_pred3_own γ φ) (at level 20).
+
+Definition vcurry {A} (Φ : list vl -d> A) : vl -d> list vl -d> A :=
+  λ v args, Φ (cons v args).
+Instance vcurry_ne A n :
+  Proper (dist n ==> (=) ==> dist n) (@vcurry A).
+Proof. solve_proper_ho. Qed.
+
+Definition vopen {A : ofeT} (Φ : A) : list vl -d> A := λ args, Φ.
+#[global] Arguments vopen /.
+
+End SavedInterpN.
