theories/iris_extra/saved_interp_dep.v
@@ -56,15 +56,17 @@ Definition vec_fold {A} {P : nat → Type}
 Module Type SavedInterpDep (Import V : VlSortsSig).
 
 Notation envPred s Σ := (env -d> s -d> iPropO Σ).
+Notation envD Σ := (envPred vl Σ).
 Definition hoEnvPred s Σ n := vec vl n -d> envPred s Σ.
+Notation hoEnvD := (hoEnvPred vl).
+
 Definition hoEnvPredO s Σ : ofeT := sigTO (hoEnvPred s Σ).
 Definition hoEnvPredOF s : oFunctor := { n & vec vl n -d> env -d> s -d> ▶ ∙ }.
+
 Definition packedHoEnvPred s Σ : ofeT := oFunctor_apply (hoEnvPredOF s) (iPropO Σ).
+Definition packedHoEnvD Σ := packedHoEnvPred vl Σ.
 
 Definition hoD Σ n := vec vl n -d> vl -d> iPropO Σ.
-Notation hoEnvD := (hoEnvPred vl).
-Notation envD Σ := (envPred vl Σ).
-Definition packedHoEnvD Σ := packedHoEnvPred vl Σ.
 
 Notation savedHoEnvPredG s Σ := (savedAnythingG Σ (hoEnvPredOF s)).
 Notation savedHoEnvPredΣ s := (savedAnythingΣ (hoEnvPredOF s)).
